cleanup

Imp/Denot.lean
@@ -5,62 +5,63 @@ import Mathlib.Order.CompleteLattice
 import Mathlib.Data.Set.Lattice
 import Mathlib.Order.FixedPoints
 
-def SRel.id: Set (α × α) := {p | p.1 = p.2}
+-- Set relation denotational semantics,
+-- aka graph of partial function
+@[reducible]
+def SRel α β := Set (α × β)
 
-@[simp] theorem SRel.mem_id (a b: α):
+infixl:20 " →ˢ " => SRel
+
+def SRel.id: α →ˢ α := {p | p.1 = p.2}
+
+@[simp] theorem SRel.mem_id {a b: α}:
   (a, b) ∈ @id α ↔ a = b := Iff.rfl
 
-def SRel.comp (r₁ r₂: Set (α × α)): Set (α × α) :=
-  {a | ∃z, (a.1, z) ∈ r₁ ∧ (z, a.2) ∈ r₂}
+def SRel.comp (f g: α →ˢ α): α →ˢ α :=
+  {x | ∃z, (x.1, z) ∈ f ∧ (z, x.2) ∈ g}
 
 infixl:90 " ○ " => SRel.comp
 
-@[simp] theorem SRel.mem_comp (r₁ r₂: Set (α × α)):
-  a ∈ r₁ ○ r₂ ↔ (∃z, (a.1, z) ∈ r₁ ∧ (z, a.2) ∈ r₂) := Iff.rfl
+@[simp] theorem SRel.mem_comp {r₁ r₂: α →ˢ α}:
+  x ∈ r₁ ○ r₂ ↔ ∃z, (x.1, z) ∈ r₁ ∧ (z, x.2) ∈ r₂ := Iff.rfl
 
-def SRel.restrictDomain (r: Set (α × α)) (p: α → Prop): Set (α × α) :=
-  {a ∈ r | p a.1}
+def SRel.restrict (f: α →ˢ α) (s: Set α): α →ˢ α :=
+  {x ∈ f | x.1 ∈ s}
 
-infixl:90 " ⇃ " => SRel.restrictDomain
-
-@[simp] theorem SRel.mem_restrictDomain (r: Set (α × α)) (p: α → Prop):
-  a ∈ r ⇃ p ↔ a ∈ r ∧ p a.1 := Iff.rfl
-
-theorem SRel.monotone_comp [PartialOrder α]
-    (f g: α → Set (β × β)) (hf: Monotone f)
-    (hg: Monotone g):
+theorem SRel.monotone_comp [PartialOrder α] {f g: α → (β →ˢ β)}
+  (hf: Monotone f) (hg: Monotone g):
   Monotone λ x ↦ f x ○ g x :=
   λ _ _ h _ ⟨z, h₁, h₂⟩ => ⟨z, hf h h₁, hg h h₂⟩
 
-theorem SRel.monotone_restrictDomain [PartialOrder α]
-    (f : α → Set (β × β)) (p: β → Prop) (hf: Monotone f):
-  Monotone λ x ↦ f x ⇃ p :=
+theorem SRel.monotone_restrict [PartialOrder α] {f : α → (β →ˢ β)} {s: Set β}
+  (hf: Monotone f):
+  Monotone λ x ↦ restrict (f x) s :=
   λ _ _ h _ ⟨z, h₁⟩ ↦ ⟨hf h z, h₁⟩
 
-def Com.Γ (b: Bexp) (f: Set (State × State)): Set (State × State) →o Set (State × State) := {
-  toFun := (λ g ↦ (f ○ g ⇃ λ s↦b↓s) ∪ (SRel.id ⇃ λ s↦b↓s=false))
-  monotone' := by
-    apply Monotone.union
-    . apply SRel.monotone_restrictDomain
-      apply SRel.monotone_comp
-      . exact monotone_const
-      . exact monotone_id
-    . apply SRel.monotone_restrictDomain
-      exact monotone_const
+def Com.Γ (b: Bexp) (f: State →ˢ State): (State →ˢ State) →o (State →ˢ State) := {
+  toFun := λ g ↦ ((f ○ g).restrict {s | b↓s = true})
+                    ∪ (SRel.id.restrict {s | b↓s = false})
+  monotone' :=
+    Monotone.union
+    (SRel.monotone_restrict (SRel.monotone_comp monotone_const monotone_id))
+    (SRel.monotone_restrict monotone_const)
 }
 
 @[simp]
-def Com.denot: Com → Set (State × State)
+def Com.denot: Com → (State →ˢ State)
   | skip      => SRel.id
   | x ≔ a     => {s | s.2 = s.1⟦x↦a↓s.1⟧}
-  | c;;d      => denot c ○ denot d
-  | ife b c d => (denot c ⇃ λ s↦b↓s) ∪ (denot d ⇃ λ s↦b↓s=false)
-  | wle b c   => OrderHom.lfp (Γ b (denot c))
+  | c;;d      => c.denot ○ d.denot
+  | ife b c d => (c.denot.restrict {s | b↓s = true})
+                  ∪ (d.denot.restrict {s | b↓s = false})
+  | wle b c   => OrderHom.lfp (Γ b c.denot)
 
 notation (priority := high) "⟦" c "⟧" => Com.denot c
 
 #simp (⟦⟧, ⟦"x"↦5⟧⟦"x"↦1⟧) ∈ ⟦⦃x ≔ 5; if x=1 {skip} else {x ≔ 1}⦄⟧
+#simp (⟦⟧, ⟦"x"↦5⟧) ∈ ⟦⦃x ≔ 5; while x=1 {x ≔ 1}⦄⟧
 
+@[simp]
 instance Com.denot.equiv: Setoid Com where
   r c d := ⟦c⟧ = ⟦d⟧
   iseqv := {
@@ -69,8 +70,33 @@ instance Com.denot.equiv: Setoid Com where
     trans := (· ▸ ·)
   }
 
--- theorem Com.denot.cat_congr (hc: c₁ ≈ c₂) (hd: d₁ ≈ d₂):
---   (c₁;;d) ≈ (c₂;;d₂) :=
---   by
---     unfold denot
---     exact hc ▸ hd ▸ rfl
+theorem Com.denot.cat_congr (hc: c₁ ≈ c₂) (hd: d₁ ≈ d₂):
+  (c₁;;d₁) ≈ (c₂;;d₂) :=
+  by
+    simp [HasEquiv.Equiv]
+    exact hc ▸ hd ▸ rfl
+
+theorem Com.denot.ife_congr (hc: c₁ ≈ c₂) (hd: d₁ ≈ d₂):
+  (ife b c₁ d₁) ≈ (ife b c₂ d₂) :=
+  by
+    simp [HasEquiv.Equiv]
+    exact hc ▸ hd ▸ rfl
+
+theorem Com.denot.wle_congr (hc: c₁ ≈ c₂):
+  (wle b c₁) ≈ (wle b c₂) :=
+  by
+    simp [HasEquiv.Equiv]
+    exact hc ▸ rfl
+
+theorem Com.denot.cat_skipl:
+  (skip;;c) ≈ c :=
+  by simp [HasEquiv.Equiv, SRel.comp]
+
+theorem Com.denot.cat_skipr:
+  (c;;skip) ≈ c :=
+  by simp [HasEquiv.Equiv, SRel.comp]
+
+theorem Com.denot.ife_unfold:
+  ife b (c;;wle b c) skip ≈ wle b c := by
+  simp [HasEquiv.Equiv]
+  exact OrderHom.map_lfp (Γ b ⟦c⟧)
